Started : 24December2025
End : 

# Precalculus - FreeCodeCamp - Dr Linda Green (5.5 Hours-2020) :
https://www.youtube.com/watch?v=eI4an8aSsgw
## 2025-December-24 - Functions :
https://www.youtube.com/watch?v=eI4an8aSsgw&t=20
- Definition. A function is correspondence between input numbers (x-values) and out-put numbers (y-value) that sends each input number (x-value) to exactly one output number (y-value).
- Sometimes, a function is described with an equation. : $y = x^2 + 1$, which can also be written as $f(x) = x^2 + 1$ : 
- $f(2) = 2^2 + 1 = 5$ 
- $f(5) = 5^2 + 1 = 26$
- $f(a+3) = a^2 + 6a + 10$ 
- not even 2 minutes into the video and she is already talking about 'functions' as 'mothers' and how you can have infinite mothers.. - Do I really want to listen to this for 5 and a half hours?
- Sometimes a function is described as a graph instead of an equation
- Definition. The **domain** of a function is all possible **x-values.**  
- The **range** is the **y-values**.
- To find domain of a function, exclude 'x' values that make the denominator '0'. Also exclude 'x' values that make an expression inside a square root negative
## 2025-December-24 - Increasing and Decreasing Functions :
https://www.youtube.com/watch?v=eI4an8aSsgw&t=12m05s
- green line go up = positive = inceasing
- blue line go down = negative = decreasing
## 2025-December-24 - Maximums and Minimums on a Graphs :
https://www.youtube.com/watch?v=eI4an8aSsgw&t=17m35s
- **Maximum** A function f(x) has an absolute maximum at x = c if the 'y' value at 'x = c' is as big as it ever gets
- **Minimum** A function f(x) has an absolute minimum at x = c if the 'y' value at 'x = c' is as small as it ever gets
- **Global Maximum/Minimum Values** = Another word for absolute maximum/minimum values
- **Local Maximum** = If it is larger than any nearby y values
- **Local Minimum** = If it is smaller than any nearby y values
- **Relative Maximum/Minimum Values** = Another name for local minimum/maximum values
## 2025-December-24 - Even and Odd Functions :
https://www.youtube.com/watch?v=eI4an8aSsgw&t=26m40s
![[Pasted image 20251224163701.png]]
- A graph is symmetric in respect to the x axis, y axis, origin if... Not typing all that out, and describing each graph.
- **Symmetric X Axis** = Mirror Symmetry with X axis (x,y) is mirrored by the same points on (x, -y)
- **Symmetric Y Axis** = Mirror Symmetry with Y axis (x,y) is mirroed on the same point with (-x, y)
- **Symmetric Origin** = Mirror Symmetry with origin (0,0) - it has $180\degree$ degree rotational symmetry -  is mirrored by inverting it upside down and should look exactly the same, (x,y) = (-x,-y)
- **Even/Odd Functions** = Used to describe functions which graphs have certain kinds of symmetry
- **Even Function** = A graph is even if it's graph is symmetric with respect to the y-axis : (x, f(x)) is mirrored by (-x, f(-x)) : aka f(-x) = f(x) for all x values in it's domain, aka same height at 'x' and '-x'
- **Odd Function** = A graph is odd if it's graph is symmetric with respect to it's origin : (x, y) is mirrored by (-x, -y) : aka f(-x) = -f(x)
- There's no word for functions that are symmetric to the x axis - because if it is symmetric with the x-axis, it's not a function (won't pass the vertical line test)
## 2025-December-25 - Toolkit Functions :
https://www.youtube.com/watch?v=eI4an8aSsgw&t=36m15s
- $y = x$ : creates a line
- $y = x^2$ : creates a parabola
- $y = x^3$ : creates a cubic odd function
- $y = \sqrt{x}$ : creates a square root function
- $y = |x|$ : creates a 'V'
- $y = 2^x$ : creates an exponential function
- $y = \frac{1}{x}$ : creates a hyperobla odd function
- $y = \frac{1}{x^2}$ : creates an even function asymptote
- You should memorize what each function looks like for future Sean
## 2025-December-26 - Transformations of Functions : 
https://www.youtube.com/watch?v=eI4an8aSsgw&t=43m20s
- If you change the equation of a function, then the graph of the function transforms.
- $y=\sqrt{x} - 2$ : moves the graph down 2 on the y axis 
- $y= \sqrt{x-2}$ : moves the graph right (counterintuitive) on the x axis - since the equation now has to add 2 units to the graph, to get it to the right original positioning, it moves it right. 
- Rules for transformations: 
  - Numbers on the outside of the function affect the y-values and result in vertical motions. These motions are in the direction you expect.
- Numbers on the inside of the function affect the x-values and result in horizontal motions. These motions go in the opposite direction from what you expect.
- Adding results in a shift (translations)
- Multiplying results in a stretch or shrink
-  A negative sign results in a reflection
- $y = \sqrt{\frac{1}{4}x}$ : The multiplier will also be inverted, this will actually **stretch** (counterintuitive, not shrink) the graph on the horizontal axis - a vertical shrink of one half$y = \frac{1}{2} \sqrt{x}$ is the same as a horizontal stretch of $y = \sqrt{\frac{1}{4}x}$
## 2025-December-26 - Piecewise Functions :
https://www.youtube.com/watch?v=eI4an8aSsgw&t=55m50s
- A **Piecewise Function** = is a function which is defined in pieces. : 
  f(x) = 
  '$-x^2$ if $x<1$'
   '$-2x+3$ if $x \ge 1$' 
- If a piecewise function is **continuous** if one piece connects directly to another piece, if there is a jump on the points of the function, it is **not continuous, discontinuous**
## 2025-December-27 - Inverse Functions :
https://www.youtube.com/watch?v=eI4an8aSsgw&t=1h20s
- **Inverse Function** = Undoes what a function does. : 
  $f(x) = x+2$ 
  $f^{-1}(x)=x -2$ 
- Inverse functions reverse the roles of y and x.
- This is the mathematical way of saying that $f$ and $f^{-1}$ undo each other.
   $f^{-1} \circ f(x) = x$ 
  $f \circ f^{-1}(x) = x$ . 
- $\circ$ = **Function Composition Symbol** = Function composition is the process of combining two functions into a single new function by using the **output** of the first (inner) function as the **input** for the second (outer) function.
### Inverse $\neq$ Reciprocal

It is a common mistake to think $f^{-1}(x)$ means the same thing as $\frac{1}{f(x)}$. While they use similar notation, they represent entirely different mathematical concepts.

---

#### The Core Difference
| Concept        | Notation                          | Meaning                    | Goal                                  |
| :------------- | :-------------------------------- | :------------------------- | :------------------------------------ |
| **Inverse**    | $f^{-1}(x)$                       | **Reverse Mapping**        | To "undo" the action of the function. |
| **Reciprocal** | $[f(x)]^{-1}$ or $\frac{1}{f(x)}$ | **Multiplicative Inverse** | To flip the output into a fraction.   |

---

#### Numerical Comparison
Let's use a simple function $f(x) = 2x$ with an input of $x = 3$.
* **Original Output:** $f(3) = 6$

**The Inverse ($f^{-1}$)**
The inverse "reverses" $2x$ to $\frac{x}{2}$.
$$f^{-1}(6) = \frac{6}{2} = 3$$
*Result: We returned to the original input.*

**The Reciprocal ($\frac{1}{f}$)**
The reciprocal simply flips the result ($6$).
$$\frac{1}{f(3)} = \frac{1}{6}$$
*Result: We just get a fraction.*

---

> [!TIP]
> To keep your notes clear, always think: **Inverse** = "Go Backwards", **Reciprocal** = "Flip Upside Down".
### Inverse Functions: $f(x) = \frac{5-x}{3x}$

An **inverse function** $f^{-1}(x)$ reverses the effect of the original function. Essentially, if $f$ maps $x$ to $y$, then $f^{-1}$ maps $y$ back to $x$.

---

#### 1. Finding the Inverse
To find the inverse of $f(x) = \frac{5-x}{3x}$, follow these algebraic steps:

1. **Set to $y$:** $y = \frac{5-x}{3x}$
2. **Swap $x$ and $y$:** $x = \frac{5-y}{3y}$
3. **Solve for the new $y$:** $x(3y) = 5 - y$  
   $3xy + y = 5$  
   $y(3x + 1) = 5$  
   $y = \frac{5}{3x+1}$

**Result:** $$f^{-1}(x) = \frac{5}{3x+1}$$

---

#### 2. How it Works (The Composition Rule)
Inverse functions are defined by the fact that their **composition** results in the identity function $x$. In Obsidian/MathJax notation:

$$(f \circ f^{-1})(x) = x \quad \text{and} \quad (f^{-1} \circ f)(x) = x$$

#### Numerical Example:
* **Original:** If we plug $x = 1$ into $f(x)$:  
    $f(1) = \frac{5 - 1}{3(1)} = \frac{4}{3}$
* **Inverse:** If we plug that result ($\frac{4}{3}$) into $f^{-1}(x)$:  
    $f^{-1}(\frac{4}{3}) = \frac{5}{3(\frac{4}{3}) + 1} = \frac{5}{4 + 1} = \frac{5}{5} = \mathbf{1}$

The inverse successfully "undid" the original operation and returned us to our starting value.
