## 2025-December-04 - Factoring Trinomials With Leading Coefficient not 1 - AC Method & By Grouping - Algebra - 3 Terms : 
https://www.youtube.com/watch?v=4v-EQIxqpMQ
- For the **AC Method** Whenever You are trying to factor by grouping and you can't see a GCF to take out, you can just use '1'
### Factoring $6x^2 + 11x - 10$ using the AC Method

* **1. Identify Coefficients**
    * The trinomial is in the form $ax^2 + bx + c$.
    * $a = 6$
    * $b = 11$
    * $c = -10$

* **2. Calculate the AC Product**
    * $A \cdot C = (6) \cdot (-10) = \mathbf{-60}$

* **3. Find Factors of AC that Sum to B**
    * We need two numbers, $p$ and $q$, such that:
        * $p \cdot q = -60$
        * $p + q = 11$
    * Since the product is negative, one factor is positive and one is negative. Since the sum (11) is positive, the larger factor must be positive.
    * The factors are: **$15$ and $-4$** ($15 + (-4) = 11$ and $15 \cdot (-4) = -60$).

* **4. Rewrite the Middle Term ($11x$)**
    * Replace $11x$ with the two new terms, $15x$ and $-4x$.
    * $6x^2 \mathbf{+ 15x - 4x} - 10$

* **5. Factor by Grouping**
    * Group the first two terms and the last two terms.
    * $(6x^2 + 15x) + (-4x - 10)$
    * Factor out the Greatest Common Factor (GCF) from each group.
        * $\text{GCF}(6x^2, 15x) = 3x \implies 3x(2x + 5)$
        * $\text{GCF}(-4x, -10) = -2 \implies -2(2x + 5)$
    * $3x(2x + 5) - 2(2x + 5)$

* **6. Factor out the Common Binomial**
    * Factor out the common binomial term $(2x + 5)$.
    * **$(2x + 5)(3x - 2)$**

#### Final Answer

The factored form of $6x^2 + 11x - 10$ is **$(2x + 5)(3x - 2)$**.

#### Check

* $(2x)(3x) + (2x)(-2) + (5)(3x) + (5)(-2)$
* $6x^2 - 4x + 15x - 10$
* $6x^2 + 11x - 10$ (Original expression confirmed)
## 2025-December-04 : How To Factor Polynomials The Easy Way! :
